proof/invariant-abstract/ARM/ArchKHeap_AI.thy
@@ -821,9 +821,37 @@ lemma state_hyp_refs_of_ntfn_update: "\<And>s ep val. typ_at ANTFN ep s \<Longri
   apply (clarsimp simp add: ARM.state_hyp_refs_of_def obj_at_def ARM.hyp_refs_of_def)
   done
 
+lemma state_hyp_refs_of_sc_update: "\<And>s sc val. typ_at ASchedContext sc s \<Longrightarrow>
+       state_hyp_refs_of (s\<lparr>kheap := kheap s(sc \<mapsto> SchedContext val)\<rparr>) = state_hyp_refs_of s"
+  apply (rule all_ext)
+  apply (clarsimp simp add: ARM.state_hyp_refs_of_def obj_at_def ARM.hyp_refs_of_def)
+  done
+
+lemma state_hyp_refs_of_reply_update: "\<And>s r val. typ_at AReply r s \<Longrightarrow>
+       state_hyp_refs_of (s\<lparr>kheap := kheap s(r \<mapsto> Reply val)\<rparr>) = state_hyp_refs_of s"
+  apply (rule all_ext)
+  apply (clarsimp simp add: ARM.state_hyp_refs_of_def obj_at_def ARM.hyp_refs_of_def)
+  done
+
 lemma state_hyp_refs_of_tcb_bound_ntfn_update:
        "kheap s t = Some (TCB tcb) \<Longrightarrow>
           state_hyp_refs_of (s\<lparr>kheap := kheap s(t \<mapsto> TCB (tcb\<lparr>tcb_bound_notification := ntfn\<rparr>))\<rparr>)
+            = state_hyp_refs_of s"
+  apply (rule all_ext)
+  apply (clarsimp simp add: ARM.state_hyp_refs_of_def obj_at_def split: option.splits)
+  done
+
+lemma state_hyp_refs_of_tcb_sched_context_update:
+       "kheap s t = Some (TCB tcb) \<Longrightarrow>
+          state_hyp_refs_of (s\<lparr>kheap := kheap s(t \<mapsto> TCB (tcb\<lparr>tcb_sched_context := sc\<rparr>))\<rparr>)
+            = state_hyp_refs_of s"
+  apply (rule all_ext)
+  apply (clarsimp simp add: ARM.state_hyp_refs_of_def obj_at_def split: option.splits)
+  done
+
+lemma state_hyp_refs_of_tcb_reply_update:
+       "kheap s t = Some (TCB tcb) \<Longrightarrow>
+          state_hyp_refs_of (s\<lparr>kheap := kheap s(t \<mapsto> TCB (tcb\<lparr>tcb_reply := reply\<rparr>))\<rparr>)
             = state_hyp_refs_of s"
   apply (rule all_ext)
   apply (clarsimp simp add: ARM.state_hyp_refs_of_def obj_at_def split: option.splits)
