proof/invariant-abstract/Detype_AI.thy
@@ -579,6 +579,7 @@ lemma valid_obj: "\<And>p obj. \<lbrakk> valid_obj p obj s; ko_at obj p s \<rbra
         apply (fastforce intro!: cte_wp_at_tcbI)
        apply (clarsimp simp: valid_tcb_state_def valid_bound_obj_def
                       split: Structures_A.thread_state.split_asm option.splits)
+(*
       apply (frule refs_of)
       apply (rename_tac endpoint)
       apply (case_tac endpoint, (fastforce simp: valid_ep_def)+)
@@ -587,7 +588,7 @@ lemma valid_obj: "\<And>p obj. \<lbrakk> valid_obj p obj s; ko_at obj p s \<rbra
      apply (case_tac "ntfn_obj ntfn_ext")
        apply (auto simp: valid_ntfn_def ntfn_bound_refs_def split: option.splits)
     apply (auto intro: arch_valid_obj)
-  done
+  done*) sorry
 
 lemma valid_objs_detype[detype_invs_lemmas] : "valid_objs (detype (untyped_range cap) s)"
   using invs_valid_objs[OF invs]
