proof/invariant-abstract/RealTime_AI.thy
@@ -1,0 +1,190 @@
+(*
+ * Copyright 2016, Data61, CSIRO
+ *
+ * This software may be distributed and modified according to the terms of
+ * the GNU General Public License version 2. Note that NO WARRANTY is provided.
+ * See "LICENSE_GPLv2.txt" for details.
+ *
+ * @TAG(DATA61_GPL)
+ *)
+
+theory RealTime_AI
+imports VSpace_AI
+begin
+
+crunch invs[wp]: get_sched_context invs
+crunch invs[wp]: get_reply invs
+
+crunch invs[wp]: get_sched_context invs
+crunch invs[wp]: get_sched_context invs
+
+lemma refs_in_get_refs:
+  "(x, ref) \<in> get_refs REF ntfn \<Longrightarrow> ref = REF"
+  by (auto simp: get_refs_def split: option.splits)
+
+crunch irq_node[wp]: set_reply "\<lambda>s. P (interrupt_irq_node s)"
+  (simp: get_object_def)
+
+lemma reply_remove_irq_node[wp]: "\<lbrace>\<lambda>s. P (interrupt_irq_node s)\<rbrace>
+  reply_remove r \<lbrace>\<lambda>_ s. P (interrupt_irq_node s)\<rbrace> "
+  sorry
+
+
+crunch interrupt_states[wp]: set_sched_context "\<lambda>s. P (interrupt_states s)"
+  (simp: get_object_def)
+
+lemma reply_remove_interrupt_states[wp]: "\<lbrace>\<lambda>s. P (interrupt_states s)\<rbrace>
+  reply_remove r \<lbrace>\<lambda>_ s. P (interrupt_states s)\<rbrace> "
+  sorry
+
+lemma reply_remove_caps_of_state[wp]:
+  "\<lbrace>\<lambda>s. P (caps_of_state s)\<rbrace> reply_remove r \<lbrace>\<lambda>rv s. P (caps_of_state s)\<rbrace>"
+  sorry
+
+crunch irq_node[wp]: set_reply "\<lambda>s. P (interrupt_irq_node s)"
+  (simp: get_object_def)
+
+lemmas reply_remove_valid_irq_nodes[wp]
+    = valid_irq_handlers_lift [OF reply_remove_caps_of_state
+                                  reply_remove_interrupt_states]
+
+lemma reply_remove_pspace_in_kernel_window[wp]:
+      "\<lbrace>pspace_in_kernel_window\<rbrace> reply_remove r
+      \<lbrace>\<lambda>r. pspace_in_kernel_window\<rbrace>"
+  sorry
+
+lemma reply_remove_pspace_respects_device_region[wp]:
+      "\<lbrace>pspace_respects_device_region\<rbrace> reply_remove r
+      \<lbrace>\<lambda>r. pspace_respects_device_region\<rbrace>"
+  sorry
+
+lemma reply_remove_cap_refs_in_kernel_window[wp]:
+      "\<lbrace>cap_refs_in_kernel_window\<rbrace> reply_remove r
+      \<lbrace>\<lambda>r. cap_refs_in_kernel_window\<rbrace>"
+  sorry
+
+
+lemma reply_remove_valid_mdb[wp]:
+      "\<lbrace>valid_mdb\<rbrace> reply_remove r
+      \<lbrace>\<lambda>r. valid_mdb\<rbrace>"
+  sorry
+
+lemma reply_remove_valid_global_refs[wp]:
+      "\<lbrace>valid_global_refs\<rbrace> reply_remove r
+      \<lbrace>\<lambda>r. valid_global_refs\<rbrace>"
+   sorry
+
+crunch arch [wp]: set_reply "\<lambda>s. P (arch_state s)"
+  (simp: get_object_def)
+
+lemma reply_remove_arch[wp]:
+      "\<lbrace>\<lambda>s. P (arch_state s)\<rbrace> reply_remove r
+      \<lbrace>\<lambda>r. \<lambda>s. P (arch_state s)\<rbrace>"
+  sorry
+
+
+lemma reply_remove_valid_objs [wp]:
+  "\<lbrace>valid_objs and reply_at r\<rbrace> reply_remove r \<lbrace>\<lambda>_. valid_objs\<rbrace>"
+  sorry
+
+lemma reply_remove_pspace_aligned[wp]:
+      "\<lbrace>pspace_aligned\<rbrace> reply_remove r
+      \<lbrace>\<lambda>r. pspace_aligned\<rbrace>"
+  sorry
+
+lemma reply_remove_tcb_at[wp]:
+      "\<lbrace>tcb_at t\<rbrace> reply_remove r
+      \<lbrace>\<lambda>r. tcb_at t\<rbrace>"
+  sorry
+
+lemma reply_remove_cte_wp_at [wp]:
+  "\<lbrace>cte_wp_at P c\<rbrace> reply_remove r \<lbrace>\<lambda>rv. cte_wp_at P c\<rbrace>"
+  sorry
+
+lemma reply_remove_distinct [wp]:
+  "\<lbrace>pspace_distinct\<rbrace> reply_remove r \<lbrace>\<lambda>_. pspace_distinct\<rbrace>"
+  sorry
+
+lemma reply_remove_cur_tcb [wp]:
+  "\<lbrace>cur_tcb\<rbrace> reply_remove r \<lbrace>\<lambda>_. cur_tcb\<rbrace>"
+  sorry
+
+lemma reply_remove_ifunsafe[wp]:
+  "\<lbrace>if_unsafe_then_cap\<rbrace> reply_remove r \<lbrace>\<lambda>rv. if_unsafe_then_cap\<rbrace>"
+  sorry
+
+lemma reply_remove_zombies[wp]:
+  "\<lbrace>zombies_final\<rbrace> reply_remove r \<lbrace>\<lambda>rv. zombies_final\<rbrace>"
+  sorry
+
+lemma reply_remove_ex_nonz_cap_to[wp]:
+  "\<lbrace>ex_nonz_cap_to p\<rbrace> reply_remove r \<lbrace>\<lambda>rv. ex_nonz_cap_to p\<rbrace>"
+  by (wp ex_nonz_cap_to_pres)
+
+lemma reply_remove_iflive[wp]:
+  "\<lbrace>\<lambda>s. if_live_then_nonz_cap s\<rbrace>
+  reply_remove r
+  \<lbrace>\<lambda>_ s. if_live_then_nonz_cap s\<rbrace>"
+  sorry
+
+lemma reply_remove_valid_ioc[wp]:
+      "\<lbrace>valid_ioc\<rbrace> reply_remove r
+      \<lbrace>\<lambda>r. valid_ioc\<rbrace>"
+  sorry
+
+(*
+lemma reply_remove_[wp]:
+      "\<lbrace>\<rbrace> reply_remove r
+      \<lbrace>\<lambda>r. \<rbrace>"
+*)
+lemma set_sched_context_invs[wp]:
+  "\<lbrace> invs and sc_at sc_ptr \<rbrace>
+      set_sched_context sc_ptr sc \<lbrace> \<lambda>_. invs \<rbrace>"
+  apply (wpsimp simp: set_object_def set_sched_context_def)
+  sorry
+
+lemma set_reply_invs[wp]:
+  "\<lbrace> invs and reply_at sc_ptr \<rbrace>
+      set_reply rptr reply \<lbrace> \<lambda>_. invs \<rbrace>"
+  apply (simp add: set_reply_def)
+  sorry
+
+
+lemma reply_unbind_sc_invs:
+  "\<lbrace> invs and sc_at sc_ptr and reply_at rptr \<rbrace>
+      reply_unbind_sc sc_ptr rptr \<lbrace> \<lambda>_. invs \<rbrace>"
+  apply (wpsimp simp: reply_unbind_sc_def)
+  sorry
+
+lemma sched_context_unbind_tcb_invs:
+  "\<lbrace> invs and sc_at sc_ptr \<rbrace>
+      sched_context_unbind_tcb sc_ptr \<lbrace> \<lambda>_. invs \<rbrace>"
+  apply (simp add: sched_context_unbind_tcb_def)
+  sorry
+
+lemma sched_context_donate_invs:
+  "\<lbrace> invs and sc_at sc_ptr and tcb_at tptr \<rbrace>
+      sched_context_donate sc_ptr tptr \<lbrace> \<lambda>_. invs \<rbrace>"
+  apply (simp add: sched_context_donate_def)
+  sorry
+
+lemma reply_unbind_caller_invs[wp]:
+  "\<lbrace> invs and tcb_at tptr and reply_at rptr \<rbrace>
+      reply_unbind_caller tptr tptr \<lbrace> \<lambda>_. invs \<rbrace>"
+  apply (wpsimp simp: reply_unbind_caller_def)
+  sorry
+
+lemma reply_remove_invs:
+  "\<lbrace> invs and reply_at r \<rbrace> reply_remove r \<lbrace> \<lambda>_. invs \<rbrace>"
+  apply (wpsimp simp: reply_remove_def | wpc)+
+  sorry
+
+
+lemma reply_push_invs:
+  "\<lbrace> invs and reply_at r and tcb_at caller and tcb_at callee\<rbrace>
+      reply_push caller callee rptr b \<lbrace> \<lambda>_. invs \<rbrace>"
+  apply (wpsimp simp: reply_push_def)
+  sorry
+
+
+end
